Main.lean
@@ -1,4 +1,0 @@
-import SPos
-
-def main : IO Unit :=
-  IO.println s!"Hello, world!"
